Add stable fresh operator.

Fresh.v
@@ -30,7 +30,6 @@ Definition least_fresh (lv:set var) : var :=
                  (fun n x => if [n ∈ lv] then x else n) in
   vx.
 
-
 Definition fresh (s : set var) : var :=
   S(fold max s 0).
 
@@ -58,6 +57,17 @@ Proof.
   intro. unfold fresh in H.
   pose proof (fresh_spec' H). omega.
 Qed.
+
+Definition fresh_stable (lv:set var) (x:var) : var :=
+  if [x ∉ lv] then x else
+    fresh lv.
+
+Lemma fresh_stable_spec G x
+      : fresh_stable G x ∉ G.
+Proof.
+  unfold fresh_stable. destruct if; eauto using fresh_spec.
+Qed.
+
 
 Fixpoint fresh_list (G:set var) (n:nat) : list var :=
   match n with
@@ -98,6 +108,36 @@ Proof.
   eapply (not_in_empty (fresh G)).
   eapply fresh_list_spec.
   cset_tac. eapply InA_in; eauto.
+  cset_tac; eauto.
+Qed.
+
+Fixpoint fresh_stable_list (G:set var) (Z:list var) : list var :=
+  match Z with
+    | nil => nil
+    | x::Z' => let x' := fresh_stable G x in x'::fresh_stable_list (G ∪ {{x'}}) Z'
+  end.
+
+
+Lemma fresh_stable_list_spec 
+: forall (G:set var) Z, (of_list (fresh_stable_list G Z)) ∩ G [=] ∅.
+Proof.
+  intros. general induction Z; simpl; split; intros.
+  - cset_tac; eauto. 
+  - exfalso; cset_tac; eauto.  
+  - cset_tac; intuition.
+    + hnf in H; subst. eapply fresh_stable_spec; eauto.
+    + specialize (IHZ (G ∪ {{fresh_stable G a}})). intuition (cset_tac; eauto).
+  - exfalso; cset_tac; auto.
+Qed.
+
+Lemma fresh_stable_list_unique (G: set var) n
+  : unique (fresh_stable_list G n).
+Proof.
+  general induction n; simpl; eauto.
+  split; eauto. intro.
+  eapply (not_in_empty (fresh_stable G a)).
+  eapply fresh_stable_list_spec.
+  cset_tac. eapply InA_in; eauto. 
   cset_tac; eauto.
 Qed.
 
